Do not make key coercions unlockable.

core/term/base.v
@@ -31,47 +31,41 @@ Record senc_key := SEncKey {
 }.
 Set Elimination Schemes.
 
-Definition term_of_aenc_key_def sk :=
-  match sk with
-  | AEncKey seed => TKey ADec seed
-  end.
+Definition term_of_aenc_key_def sk := TKey ADec (seed_of_aenc_key sk).
 Fact term_of_aenc_key_key : unit. exact: tt. Qed.
 Definition term_of_aenc_key :=
   locked_with term_of_aenc_key_key term_of_aenc_key_def.
-Canonical unlockable_term_of_aenc_key :=
-  [unlockable of term_of_aenc_key].
+Lemma term_of_aenc_keyE : term_of_aenc_key = term_of_aenc_key_def.
+Proof. exact: locked_withE. Qed.
 Coercion term_of_aenc_key : aenc_key >-> term.
 
-Lemma term_of_aenc_key_inj : injective term_of_aenc_key.
-Proof. rewrite unlock. by case=> [?] [?] [->]. Qed.
-
-Definition term_of_sign_key_def sk :=
-  match sk with
-  | SignKey seed => TKey Sign seed
-  end.
+Definition term_of_sign_key_def sk := TKey Sign (seed_of_sign_key sk).
 Fact term_of_sign_key_key : unit. exact: tt. Qed.
 Definition term_of_sign_key :=
   locked_with term_of_sign_key_key term_of_sign_key_def.
-Canonical unlockable_term_of_sign_key :=
-  [unlockable of term_of_sign_key].
+Lemma term_of_sign_keyE : term_of_sign_key = term_of_sign_key_def.
+Proof. exact: locked_withE. Qed.
 Coercion term_of_sign_key : sign_key >-> term.
 
-Lemma term_of_sign_key_inj : injective term_of_sign_key.
-Proof. rewrite unlock. by case=> [?] [?] [->]. Qed.
-
-Definition term_of_senc_key_def sk :=
-  match sk with
-  | SEncKey seed => TKey SEnc seed
-  end.
+Definition term_of_senc_key_def sk := TKey SEnc (seed_of_senc_key sk).
 Fact term_of_senc_key_key : unit. exact: tt. Qed.
 Definition term_of_senc_key :=
   locked_with term_of_senc_key_key term_of_senc_key_def.
-Canonical unlockable_term_of_senc_key :=
-  [unlockable of term_of_senc_key].
+Lemma term_of_senc_keyE : term_of_senc_key = term_of_senc_key_def.
+Proof. exact: locked_withE. Qed.
 Coercion term_of_senc_key : senc_key >-> term.
 
+Definition keysE :=
+  (term_of_aenc_keyE, term_of_sign_keyE, term_of_senc_keyE).
+
+Lemma term_of_aenc_key_inj : injective term_of_aenc_key.
+Proof. rewrite keysE. by case=> [?] [?] [->]. Qed.
+
+Lemma term_of_sign_key_inj : injective term_of_sign_key.
+Proof. rewrite keysE. by case=> [?] [?] [->]. Qed.
+
 Lemma term_of_senc_key_inj : injective term_of_senc_key.
-Proof. rewrite unlock. by case=> [?] [?] [->]. Qed.
+Proof. rewrite keysE. by case=> [?] [?] [->]. Qed.
 
 (* We use a different name for the default induction scheme, as it does not
    allow us to recurse under exponentials.  Later, we'll prove term_ind, which
